src/cbor/pulse/raw/everparse/CBOR.Pulse.Raw.EverParse.ResetPerm.fst
@@ -64,12 +64,12 @@ ensures cbor_raw_match_content p pp q h (cbor_raw_reset_perm_tot (pm /. q) xl) c
         let v' : cbor_string = { v with cbor_string_perm = (pm /. q) *. v.cbor_string_perm };
         cbor_raw_match_content_eq_string p pp pm b la v c;
         rewrite (cbor_raw_match_content p pp pm (| b, la |) (CBOR_Case_String v) c)
-             as (S.pts_to v.cbor_string_ptr #(pm *. v.cbor_string_perm) (content_as_seq_u8 b la c));
+             as (S.pts_to (to_slice v.cbor_string_ptr) #(pm *. v.cbor_string_perm) (content_as_seq_u8 b la c));
         perm_q_p_r q pm v.cbor_string_perm;
-        rewrite (S.pts_to v.cbor_string_ptr #(pm *. v.cbor_string_perm) (content_as_seq_u8 b la c))
-             as (S.pts_to v'.cbor_string_ptr #(q *. v'.cbor_string_perm) (content_as_seq_u8 b la c));
+        rewrite (S.pts_to (to_slice v.cbor_string_ptr) #(pm *. v.cbor_string_perm) (content_as_seq_u8 b la c))
+             as (S.pts_to (to_slice v'.cbor_string_ptr) #(q *. v'.cbor_string_perm) (content_as_seq_u8 b la c));
         cbor_raw_match_content_eq_string p pp q b la v' c;
-        rewrite (S.pts_to v'.cbor_string_ptr #(q *. v'.cbor_string_perm) (content_as_seq_u8 b la c))
+        rewrite (S.pts_to (to_slice v'.cbor_string_ptr) #(q *. v'.cbor_string_perm) (content_as_seq_u8 b la c))
              as (cbor_raw_match_content p pp q (| b, la |) (CBOR_Case_String v') c);
         rewrite (cbor_raw_match_content p pp q (| b, la |) (CBOR_Case_String v') c)
              as (cbor_raw_match_content p pp q h (cbor_raw_reset_perm_tot (pm /. q) xl) c);
@@ -265,12 +265,12 @@ ensures cbor_raw_match_content p pp q h (cbor_raw_reset_perm_tot (pm /. q) xl) c
         let cr = content_as_raw_data_item b la c;
         cbor_raw_match_content_eq_tagged_serialized p pp pm b la v c;
         rewrite (cbor_raw_match_content p pp pm (| b, la |) (CBOR_Case_Tagged_Serialized v) c)
-             as (pts_to_parsed_strong_prefix pp v.cbor_tagged_serialized_ptr #(pm *. v.cbor_tagged_serialized_slice_perm) cr);
+             as (pts_to_parsed_strong_prefix pp (to_slice v.cbor_tagged_serialized_ptr) #(pm *. v.cbor_tagged_serialized_slice_perm) cr);
         perm_q_p_r q pm v.cbor_tagged_serialized_slice_perm;
-        rewrite (pts_to_parsed_strong_prefix pp v.cbor_tagged_serialized_ptr #(pm *. v.cbor_tagged_serialized_slice_perm) cr)
-             as (pts_to_parsed_strong_prefix pp v'.cbor_tagged_serialized_ptr #(q *. v'.cbor_tagged_serialized_slice_perm) cr);
+        rewrite (pts_to_parsed_strong_prefix pp (to_slice v.cbor_tagged_serialized_ptr) #(pm *. v.cbor_tagged_serialized_slice_perm) cr)
+             as (pts_to_parsed_strong_prefix pp (to_slice v'.cbor_tagged_serialized_ptr) #(q *. v'.cbor_tagged_serialized_slice_perm) cr);
         cbor_raw_match_content_eq_tagged_serialized p pp q b la v' c;
-        rewrite (pts_to_parsed_strong_prefix pp v'.cbor_tagged_serialized_ptr #(q *. v'.cbor_tagged_serialized_slice_perm) cr)
+        rewrite (pts_to_parsed_strong_prefix pp (to_slice v'.cbor_tagged_serialized_ptr) #(q *. v'.cbor_tagged_serialized_slice_perm) cr)
              as (cbor_raw_match_content p pp q (| b, la |) (CBOR_Case_Tagged_Serialized v') c);
         rewrite (cbor_raw_match_content p pp q (| b, la |) (CBOR_Case_Tagged_Serialized v') c)
              as (cbor_raw_match_content p pp q h (cbor_raw_reset_perm_tot (pm /. q) xl) c);
